src/impl/system.lean
@@ -87,7 +87,7 @@ def handle (ev : Event) (now : Nat) (org : Origin) : Reply × Commands :=
   match ev with
   | .external req =>
       let swept := sweep now org
-      let (res, c) := handleExternal req now (org.add swept.add).current
+      let (res, c) := handleExternal req now (swept.doc org).current
       (.external res, swept.merge c)
   | .internal _ =>
       (.internal, sweep now org)
